current/cliqueColorable.v
@@ -1,33 +1,5 @@
 Require Export ThreeSatReduction.  
-
-Theorem edgesNeq : forall eta' eta Gamma C i u u1, 
-                     u <> u1 -> In (u,3*u,3*u+1,3*u+2) Gamma -> In (u1,3*u1,3*u1+1,3*u1+2) Gamma ->
-                     setVertices Gamma C i eta' eta -> 
-                     exists c1 c2, In (3*u+2,c1) eta' /\ In (3*u1+2, c2) eta' /\ c1 <> c2 /\
-                              c1 <= C /\ c2 <= C. 
-Proof.
-  intros. genDeps {{ u;u1 }}. induction H2; intros.
-  {inCons. 
-   {inCons. invertTupEq. omega. invertTupEq. copy H2. eapply InSetVertices in H2; eauto. 
-    invertHyp. eapply geSetVertices in H1; eauto. exists u0. exists x. split. simpl. 
-    auto. split. simpl. auto. split; auto. omega. split; auto. omega. }
-   {inCons. invertTupEq. copy H2. eapply InSetVertices in H2; eauto. 
-    invertHyp. eapply geSetVertices in H1; eauto. exists x. exists u1. split. simpl. auto. split. 
-    simpl. auto. split. omega. split; auto. omega. eapply IHsetVertices in H0; eauto. 
-    invertHyp. exists x. exists x0. split. simpl. auto. split. simpl. auto. auto. }
-  }
-  {inCons. 
-   {inCons. invertTupEq. omega. invertTupEq. copy H2. eapply InSetVertices in H2; eauto. 
-    invertHyp. eapply geSetVertices in H1; eauto. exists u0. exists x. split. simpl. 
-    auto. split. simpl. auto. split; auto. omega. split; auto. omega. }
-   {inCons. invertTupEq. copy H2. eapply InSetVertices in H2; eauto. 
-    invertHyp. eapply geSetVertices in H1; eauto. exists x. exists u1. split. simpl. auto. split. 
-    simpl. auto. split. omega. split; auto. omega. eapply IHsetVertices in H0; eauto. 
-    invertHyp. exists x. exists x0. split. simpl. auto. split. simpl. auto. auto. }
-  }
-  {inv H0. }
-Qed. 
-
+ 
 Theorem connectXColorable : forall Gamma Delta G C eta eta' u, 
                               ~In u Delta -> setVertices Gamma C 0 eta' eta -> In (u,3*u,3*u+1,3*u+2) Gamma ->
                               connectX Gamma Delta (3*u+2) G -> coloring eta' G C. 
@@ -36,18 +8,19 @@ Proof.
   {constructor. } 
   {subst. destruct(eq_nat_dec u u0). 
    {subst. exfalso. apply H. simpl. auto. }
-   {copy H3. eapply edgesNeq in H3; eauto. invertHyp. econstructor; eauto.
-    eapply IHconnectX; eauto. intros c. apply H. simpl. right. auto. }
+   {copy H3. eapply XMapsToU in H0; eauto. copy H1. eapply XMapsToU in H1; eauto.
+    invertHyp. econstructor; eauto. omega. omega. eapply IHconnectX; eauto. intros c. 
+    apply H. simpl. auto. }
   }
 Qed. 
- 
-Theorem cliqueColorable : forall Gamma eta Delta C G eta' S5, 
+
+Theorem cliqueColorable : forall Gamma eta Delta C G eta' U, 
                             setVertices Gamma C 0 eta' eta -> 
-                            genericUnique S5 (fun x => x) Delta -> 
+                            unique U Delta -> 
                             clique Gamma Delta G -> coloring eta' G C. 
 Proof.
-  intros. genDeps {{ eta; C }}. induction H1; intros; auto. 
-  {constructor. eapply IHclique; eauto. inv H0. eapply genericUniqueSubset; eauto. 
-   eapply connectXColorable; eauto. inv H0. eapply genericUniqueNotIn. 
-   Focus 2. eauto. simpl. apply Union_intror. constructor. }
+  intros. genDeps {{ eta; C; U }}. induction H1; intros; auto. 
+  {constructor. eapply IHclique; eauto. inv H0. constructor. inv H2. eauto. 
+   eapply connectXColorable; eauto. inv H2. eapply uniqueNotIn; eauto. 
+   apply Union_intror. constructor. }
 Qed. 
